AwsCryptographicMaterialProviders/runtimes/net/Generated/AwsCryptographicMaterialProviders/GetHKDFProviderOutput.cs
@@ -1,0 +1,20 @@
+// Copyright Amazon.com Inc. or its affiliates. All Rights Reserved.
+// SPDX-License-Identifier: Apache-2.0
+// Do not modify this file. This file is machine generated, and any changes to it will be overwritten.
+using System;
+ using AWS.Cryptography.MaterialProviders; namespace AWS.Cryptography.MaterialProviders {
+ public class GetHKDFProviderOutput {
+ private AWS.Cryptography.Primitives.HKDFProvider _provider ;
+ public AWS.Cryptography.Primitives.HKDFProvider Provider {
+ get { return this._provider; }
+ set { this._provider = value; }
+}
+ public bool IsSetProvider () {
+ return this._provider != null;
+}
+ public void Validate() {
+ if (!IsSetProvider()) throw new System.ArgumentException("Missing value for required property 'Provider'");
+
+}
+}
+}
