AwsCryptographicMaterialProviders/runtimes/net/Generated/AwsCryptographicMaterialProviders/MaterialProviders.cs
@@ -183,5 +183,11 @@ using System;
  if (result.is_Failure) throw TypeConversion.FromDafny_CommonError(result.dtor_error);
  
 }
+ public AWS.Cryptography.Primitives.GetHKDFProviderOutput GetHKDFProvider(AWS.Cryptography.Primitives.GetHKDFProviderInput input) {
+ software.amazon.cryptography.primitives.internaldafny.types._IGetHKDFProviderInput internalInput = TypeConversion.ToDafny_N3_aws__N12_cryptography__N10_primitives__S20_GetHKDFProviderInput(input);
+ Wrappers_Compile._IResult<software.amazon.cryptography.primitives.internaldafny.types._IGetHKDFProviderOutput, software.amazon.cryptography.materialproviders.internaldafny.types._IError> result = _impl.GetHKDFProvider(internalInput);
+ if (result.is_Failure) throw TypeConversion.FromDafny_CommonError(result.dtor_error);
+ return TypeConversion.FromDafny_N3_aws__N12_cryptography__N10_primitives__S21_GetHKDFProviderOutput(result.dtor_value);
+}
 }
 }
