AwsCryptographicMaterialProviders/runtimes/net/Generated/AwsCryptographicMaterialProviders/TypeConversion.cs
@@ -852,6 +852,20 @@ throw new System.ArgumentException("Invalid AWS.Cryptography.MaterialProviders.S
 
  return new software.amazon.cryptography.materialproviders.internaldafny.types.ValidEncryptionMaterialsTransitionInput ( ToDafny_N3_aws__N12_cryptography__N17_materialProviders__S39_ValidEncryptionMaterialsTransitionInput__M5_start(value.Start) , ToDafny_N3_aws__N12_cryptography__N17_materialProviders__S39_ValidEncryptionMaterialsTransitionInput__M4_stop(value.Stop) ) ;
 }
+ internal static AWS.Cryptography.Primitives.GetHKDFProviderInput FromDafny_N3_aws__N12_cryptography__N10_primitives__S20_GetHKDFProviderInput (software.amazon.cryptography.primitives.internaldafny.types._IGetHKDFProviderInput value) {
+ software.amazon.cryptography.primitives.internaldafny.types.GetHKDFProviderInput concrete = (software.amazon.cryptography.primitives.internaldafny.types.GetHKDFProviderInput)value; AWS.Cryptography.Primitives.GetHKDFProviderInput converted = new AWS.Cryptography.Primitives.GetHKDFProviderInput();  return converted;
+}
+ internal static software.amazon.cryptography.primitives.internaldafny.types._IGetHKDFProviderInput ToDafny_N3_aws__N12_cryptography__N10_primitives__S20_GetHKDFProviderInput (AWS.Cryptography.Primitives.GetHKDFProviderInput value) {
+
+ return new software.amazon.cryptography.primitives.internaldafny.types.GetHKDFProviderInput (  ) ;
+}
+ internal static AWS.Cryptography.Primitives.GetHKDFProviderOutput FromDafny_N3_aws__N12_cryptography__N10_primitives__S21_GetHKDFProviderOutput (software.amazon.cryptography.primitives.internaldafny.types._IGetHKDFProviderOutput value) {
+ software.amazon.cryptography.primitives.internaldafny.types.GetHKDFProviderOutput concrete = (software.amazon.cryptography.primitives.internaldafny.types.GetHKDFProviderOutput)value; AWS.Cryptography.Primitives.GetHKDFProviderOutput converted = new AWS.Cryptography.Primitives.GetHKDFProviderOutput();  converted.Provider = (AWS.Cryptography.Primitives.HKDFProvider) FromDafny_N3_aws__N12_cryptography__N10_primitives__S21_GetHKDFProviderOutput__M8_provider(concrete._provider); return converted;
+}
+ internal static software.amazon.cryptography.primitives.internaldafny.types._IGetHKDFProviderOutput ToDafny_N3_aws__N12_cryptography__N10_primitives__S21_GetHKDFProviderOutput (AWS.Cryptography.Primitives.GetHKDFProviderOutput value) {
+
+ return new software.amazon.cryptography.primitives.internaldafny.types.GetHKDFProviderOutput ( ToDafny_N3_aws__N12_cryptography__N10_primitives__S21_GetHKDFProviderOutput__M8_provider(value.Provider) ) ;
+}
  internal static AWS.Cryptography.MaterialProviders.ESDKAlgorithmSuiteId FromDafny_N3_aws__N12_cryptography__N17_materialProviders__S16_AlgorithmSuiteId__M4_ESDK (software.amazon.cryptography.materialproviders.internaldafny.types._IESDKAlgorithmSuiteId value) {
  return FromDafny_N3_aws__N12_cryptography__N17_materialProviders__S20_ESDKAlgorithmSuiteId(value);
 }
@@ -1866,6 +1880,12 @@ throw new System.ArgumentException("Invalid AWS.Cryptography.MaterialProviders.S
  internal static software.amazon.cryptography.materialproviders.internaldafny.types._IEncryptionMaterials ToDafny_N3_aws__N12_cryptography__N17_materialProviders__S39_ValidEncryptionMaterialsTransitionInput__M4_stop (AWS.Cryptography.MaterialProviders.EncryptionMaterials value) {
  return ToDafny_N3_aws__N12_cryptography__N17_materialProviders__S19_EncryptionMaterials(value);
 }
+ internal static AWS.Cryptography.Primitives.HKDFProvider FromDafny_N3_aws__N12_cryptography__N10_primitives__S21_GetHKDFProviderOutput__M8_provider (software.amazon.cryptography.primitives.internaldafny.types._IHKDFProvider value) {
+ return FromDafny_N3_aws__N12_cryptography__N10_primitives__S12_HKDFProvider(value);
+}
+ internal static software.amazon.cryptography.primitives.internaldafny.types._IHKDFProvider ToDafny_N3_aws__N12_cryptography__N10_primitives__S21_GetHKDFProviderOutput__M8_provider (AWS.Cryptography.Primitives.HKDFProvider value) {
+ return ToDafny_N3_aws__N12_cryptography__N10_primitives__S12_HKDFProvider(value);
+}
  internal static System.IO.MemoryStream FromDafny_N6_smithy__N3_api__S4_Blob (Dafny.ISequence<byte> value) {
  return new System.IO.MemoryStream(value.Elements);
 }
@@ -2224,6 +2244,16 @@ throw new System.ArgumentException("Invalid AWS.Cryptography.Primitives.DigestAl
  if (AWS.Cryptography.Primitives.DigestAlgorithm.SHA_384.Equals(value)) return software.amazon.cryptography.primitives.internaldafny.types.DigestAlgorithm.create_SHA__384();
  if (AWS.Cryptography.Primitives.DigestAlgorithm.SHA_256.Equals(value)) return software.amazon.cryptography.primitives.internaldafny.types.DigestAlgorithm.create_SHA__256();
 throw new System.ArgumentException("Invalid AWS.Cryptography.Primitives.DigestAlgorithm value");
+}
+ internal static AWS.Cryptography.Primitives.HKDFProvider FromDafny_N3_aws__N12_cryptography__N10_primitives__S12_HKDFProvider (software.amazon.cryptography.primitives.internaldafny.types._IHKDFProvider value) {
+ if (value.is_ACCP) return AWS.Cryptography.Primitives.HKDFProvider.ACCP;
+ if (value.is_MPL) return AWS.Cryptography.Primitives.HKDFProvider.MPL;
+throw new System.ArgumentException("Invalid AWS.Cryptography.Primitives.HKDFProvider value");
+}
+ internal static software.amazon.cryptography.primitives.internaldafny.types._IHKDFProvider ToDafny_N3_aws__N12_cryptography__N10_primitives__S12_HKDFProvider (AWS.Cryptography.Primitives.HKDFProvider value) {
+ if (AWS.Cryptography.Primitives.HKDFProvider.ACCP.Equals(value)) return software.amazon.cryptography.primitives.internaldafny.types.HKDFProvider.create_ACCP();
+ if (AWS.Cryptography.Primitives.HKDFProvider.MPL.Equals(value)) return software.amazon.cryptography.primitives.internaldafny.types.HKDFProvider.create_MPL();
+throw new System.ArgumentException("Invalid AWS.Cryptography.Primitives.HKDFProvider value");
 }
  internal static int FromDafny_N3_aws__N12_cryptography__N17_materialProviders__S12_DefaultCache__M13_entryCapacity (int value) {
  return FromDafny_N3_aws__N12_cryptography__N17_materialProviders__S14_CountingNumber(value);
